Equiv.v
@@ -4,44 +4,74 @@
 Require Import RelationClasses Arith Omega Defs Proofs.
 Require Nam Mix.
 Import ListNotations.
+Import Nam Nam.Form.
 Local Open Scope bool_scope.
 Local Open Scope lazy_bool_scope.
 Local Open Scope eqb_scope.
 
+(** From named to locally nameless *)
+
 Fixpoint nam2mix_term stack t :=
   match t with
-  | Nam.Var v =>
+  | Var v =>
     match list_index v stack with
     | None => Mix.FVar v
     | Some n => Mix.BVar n
     end
-  | Nam.Fun f args =>
+  | Fun f args =>
     Mix.Fun f (List.map (nam2mix_term stack) args)
   end.
 
 Fixpoint nam2mix stack f :=
   match f with
-  | Nam.True => Mix.True
-  | Nam.False => Mix.False
-  | Nam.Not f => Mix.Not (nam2mix stack f)
-  | Nam.Op o f1 f2 =>
-    Mix.Op o (nam2mix stack f1) (nam2mix stack f2)
-  | Nam.Pred p args =>
-    Mix.Pred p (List.map (nam2mix_term stack) args)
-  | Nam.Quant q v f =>
-    Mix.Quant q (nam2mix (v::stack) f)
+  | True => Mix.True
+  | False => Mix.False
+  | Not f => Mix.Not (nam2mix stack f)
+  | Op o f1 f2 => Mix.Op o (nam2mix stack f1) (nam2mix stack f2)
+  | Pred p args => Mix.Pred p (List.map (nam2mix_term stack) args)
+  | Quant q v f => Mix.Quant q (nam2mix (v::stack) f)
   end.
 
-Module Nam2MixProof.
+(** Opposite direction *)
 
-Inductive Inv (vars:Vars.t) : Nam.subst -> Nam.subst -> Prop :=
+Fixpoint mix2nam_term stack t :=
+  match t with
+  | Mix.FVar v => Var v
+  | Mix.BVar n => Var (List.nth n stack EmptyString)
+  | Mix.Fun f args => Fun f (List.map (mix2nam_term stack) args)
+  end.
+
+Fixpoint mix2nam stack f :=
+  match f with
+  | Mix.True => True
+  | Mix.False => False
+  | Mix.Not f => Not (mix2nam stack f)
+  | Mix.Op o f1 f2 => Op o (mix2nam stack f1) (mix2nam stack f2)
+  | Mix.Pred p args => Pred p (List.map (mix2nam_term stack) args)
+  | Mix.Quant q f =>
+    let v := fresh_var (Vars.union (vars_of_list stack) (Mix.fvars f)) in
+    Nam.Quant q v (mix2nam (v::stack) f)
+  end.
+
+(** First, we prove that [nam2mix] is canonical :
+    it sends alpha-equivalent named formulas to equal mixed formulas. *)
+
+(** The invariant used during the proof *)
+
+Module Nam2Mix.
+
+Inductive Inv (vars:Vars.t) : Subst.t -> Subst.t -> Prop :=
  | InvNil : Inv vars [] []
  | InvCons v v' z sub sub' :
    Inv vars sub sub' ->
    ~Vars.In z vars ->
-   ~Vars.In z (Nam.subvars sub) ->
-   ~Vars.In z (Nam.subvars sub') ->
-   Inv vars ((v,Nam.Var z)::sub) ((v',Nam.Var z)::sub').
+   ~Vars.In z (Nam.Subst.vars sub) ->
+   ~Vars.In z (Nam.Subst.vars sub') ->
+   Inv vars ((v,Var z)::sub) ((v',Var z)::sub').
+
+End Nam2Mix.
+Import Nam2Mix.
+
 Hint Constructors Inv.
 
 Lemma Inv_sym vars sub sub' :
@@ -52,11 +82,9 @@ Qed.
 
 Lemma Inv_notIn sub sub' vars v :
  Inv vars sub sub' ->
-  ~(Vars.In v vars /\ Vars.In v (Nam.suboutvars sub)).
+  ~(Vars.In v vars /\ Vars.In v (Subst.outvars sub)).
 Proof.
- induction 1.
- - unfold Nam.subvars. simpl. varsdec.
- - unfold Nam.subvars in *. simpl. varsdec.
+ induction 1; unfold Subst.vars in *; simpl; varsdec.
 Qed.
 
 Lemma Inv_weak sub sub' vars vars' :
@@ -67,7 +95,7 @@ Qed.
 
 Lemma Inv_listassoc_var vars sub sub' :
   Inv vars sub sub' ->
-  forall v t, list_assoc v sub = Some t -> exists z, t = Nam.Var z.
+  forall v t, list_assoc v sub = Some t -> exists z, t = Var z.
 Proof.
  induction 1.
  - easy.
@@ -77,7 +105,7 @@ Proof.
 Qed.
 
 Lemma list_assoc_some_in v sub z :
-  list_assoc v sub = Some (Nam.Var z) -> Vars.In z (Nam.suboutvars sub).
+  list_assoc v sub = Some (Var z) -> Vars.In z (Subst.outvars sub).
 Proof.
  induction sub as [|(v',t) sub IH]; try easy.
  simpl.
@@ -88,8 +116,8 @@ Qed.
 
 Lemma list_assoc_index vars v v' sub sub' z :
 Inv vars sub sub' ->
-list_assoc v sub = Some (Nam.Var z) ->
-list_assoc v' sub' = Some (Nam.Var z) ->
+list_assoc v sub = Some (Var z) ->
+list_assoc v' sub' = Some (Var z) ->
 exists k,
 list_index v (map fst sub) = Some k /\
 list_index v' (map fst sub') = Some k.
@@ -99,9 +127,9 @@ Proof.
  do 2 case eqbspec.
  - intros. now exists 0.
  - intros NE <- [= <-] E. apply list_assoc_some_in in E.
-   unfold Nam.subvars in *. varsdec.
+   unfold Nam.Subst.vars in *. varsdec.
  - intros <- NE E [= <-]. apply list_assoc_some_in in E.
-   unfold Nam.subvars in *. varsdec.
+   unfold Nam.Subst.vars in *. varsdec.
  - intros _ _ E E'. destruct (IHInv E E') as (k & Hk & Hk').
    exists (S k). simpl in *. now rewrite Hk, Hk'.
 Qed.
@@ -133,178 +161,102 @@ Proof.
 Qed.
 
 Lemma nam2mix_term_ok sub sub' t t' :
- Inv (Vars.union (Nam.term_vars t) (Nam.term_vars t')) sub sub' ->
- Nam.term_substs sub t = Nam.term_substs sub' t' ->
+ Inv (Vars.union (Term.vars t) (Term.vars t')) sub sub' ->
+ Term.substs sub t = Term.substs sub' t' <->
  nam2mix_term (map fst sub) t = nam2mix_term (map fst sub') t'.
 Proof.
  revert t t' sub sub'.
  fix IH 1. destruct t as [v|f a], t' as [v'|f' a']; intros sub sub' inv;
    simpl; rewrite ?list_assoc_dft_alt.
- - simpl in *.
-   destruct (list_assoc v sub) eqn:E, (list_assoc v' sub') eqn:E'.
-   + intros <-.
-     destruct (Inv_listassoc_var _ _ _ inv v t E) as (z, ->).
-     destruct (list_assoc_index _ v v' sub sub' z inv E E') as (k & Hk & Hk').
-     simpl in Hk, Hk'.
-     now rewrite Hk, Hk'.
-   + intros ->.
-     apply list_assoc_some_in in E.
-     destruct (Inv_notIn _ _ _ v' inv). varsdec.
-   + intros <-.
-     apply list_assoc_some_in in E'.
-     apply Inv_sym in inv.
-     destruct (Inv_notIn _ _ _ v inv). varsdec.
-   + intros [= <-].
-     rewrite list_assoc_index_none in E, E'.
-     simpl in *. now rewrite E, E'.
- - generalize (Inv_listassoc_var _ _ _ inv v).
-   destruct list_assoc as [t|]; try easy.
-   intros E. destruct (E t) as (v', ->); easy.
- - apply Inv_sym in inv.
-   generalize (Inv_listassoc_var _ _ _ inv v').
-   destruct list_assoc as [t'|]; try easy.
-   intros E. destruct (E t') as (v, ->); easy.
- - intros [= <- E]. f_equal.
-   simpl in inv.
-   clear f. revert a a' E inv.
-   fix IH' 1. destruct a as [|t a], a' as [|t' a']; try easy.
-   simpl.
-   intros [= E E'] inv. f_equal.
-   + apply IH; auto.
-     eapply Inv_weak; eauto. varsdec.
-   + apply IH'; auto.
-     eapply Inv_weak; eauto. varsdec.
+ - simpl in *. split.
+   + destruct (list_assoc v sub) eqn:E, (list_assoc v' sub') eqn:E'.
+     * intros <-.
+       destruct (Inv_listassoc_var _ _ _ inv v t E) as (z, ->).
+       destruct (list_assoc_index _ v v' sub sub' z inv E E') as (k & Hk & Hk').
+       simpl in Hk, Hk'.
+       now rewrite Hk, Hk'.
+     * intros ->.
+       apply list_assoc_some_in in E.
+       destruct (Inv_notIn _ _ _ v' inv). varsdec.
+     * intros <-.
+       apply list_assoc_some_in in E'.
+       apply Inv_sym in inv.
+       destruct (Inv_notIn _ _ _ v inv). varsdec.
+     * intros [= <-].
+       rewrite list_assoc_index_none in E, E'.
+       simpl in *. now rewrite E, E'.
+   + destruct (list_index v) eqn:E, (list_index v') eqn:E'; intros [= <-].
+     * destruct (list_index_assoc _ _ _ _ _ _ inv E E') as (k & Hk & Hk').
+       simpl in *. now rewrite Hk, Hk'.
+     * rewrite <- list_assoc_index_none in E, E'.
+       simpl in *. now rewrite E,E'.
+ - split.
+   + generalize (Inv_listassoc_var _ _ _ inv v).
+     destruct list_assoc as [t|]; try easy.
+     intros E. destruct (E t) as (v', ->); easy.
+   + destruct list_index; easy.
+ - split.
+   + apply Inv_sym in inv.
+     generalize (Inv_listassoc_var _ _ _ inv v').
+     destruct list_assoc as [t'|]; try easy.
+     intros E. destruct (E t') as (v, ->); easy.
+   + destruct list_index; easy.
+ - split. intros [= <- E]. f_equal.
+   + simpl in inv.
+     clear f. revert a a' E inv.
+     fix IH' 1. destruct a as [|t a], a' as [|t' a']; try easy.
+     simpl.
+     intros [= E E'] inv. f_equal.
+     * apply IH; auto. eapply Inv_weak; eauto. varsdec.
+     * apply IH'; auto. eapply Inv_weak; eauto. varsdec.
+   + intros [= <- E]. f_equal.
+     simpl in inv.
+     clear f. revert a a' E inv.
+     fix IH' 1. destruct a as [|t a], a' as [|t' a']; try easy.
+     simpl.
+     intros [= E E'] inv. f_equal.
+     * apply IH; auto. eapply Inv_weak; eauto. varsdec.
+     * apply IH'; auto. eapply Inv_weak; eauto. varsdec.
 Qed.
 
 Lemma nam2mix_canonical_gen sub sub' f f' :
- Inv (Vars.union (Nam.allvars f) (Nam.allvars f')) sub sub' ->
- Nam.alpha_equiv_gen sub f sub' f' = true ->
+ Inv (Vars.union (allvars f) (allvars f')) sub sub' ->
+ αeq_gen sub f sub' f' = true <->
  nam2mix (List.map fst sub) f = nam2mix (List.map fst sub') f'.
 Proof.
  revert f' sub sub'.
- induction f; destruct f'; intros sub sub'; simpl; try easy.
- - case eqbspec; [ intros <- | easy ].
-   case eqbspec; try discriminate.
-   intros H inv _.
-   f_equal.
-   injection (nam2mix_term_ok sub sub' (Nam.Fun "" l) (Nam.Fun "" l0)); auto.
-   simpl. now f_equal.
- - intros. f_equal. auto.
- - case eqbspec; [ intros <- | easy].
-   rewrite lazy_andb_iff. intros E (H,H'); f_equal.
-   + apply IHf1; auto. eapply Inv_weak; eauto; varsdec.
-   + apply IHf2; auto. eapply Inv_weak; eauto; varsdec.
- - match goal with
-     |- context [fresh_var ?vs] => set (vars := vs)
-   end.
-   case eqbspec; [intros <- | easy].
-   intros inv H. f_equal. apply IHf in H; auto. clear H.
-   assert (Fok := fresh_var_ok vars).
-   constructor; try (eapply Inv_weak; eauto); varsdec.
-Qed.
-
-Lemma nam2mix_canonical f f' :
- Nam.AlphaEq f f' -> nam2mix [] f = nam2mix [] f'.
-Proof.
- intros H.
- unfold Nam.AlphaEq, Nam.alpha_equiv in *.
- apply nam2mix_canonical_gen in H; auto.
-Qed.
-
-Lemma nam2mix_term_ok2 sub sub' t t' :
- Inv (Vars.union (Nam.term_vars t) (Nam.term_vars t')) sub sub' ->
- nam2mix_term (map fst sub) t = nam2mix_term (map fst sub') t' ->
- Nam.term_substs sub t = Nam.term_substs sub' t'.
-Proof.
- revert t t' sub sub'.
- fix IH 1. destruct t as [v|f a], t' as [v'|f' a']; intros sub sub' inv;
-   simpl; rewrite ?list_assoc_dft_alt.
- - simpl in *.
-   destruct (list_index v) eqn:E, (list_index v') eqn:E';
-   intros [= <-].
-   + destruct (list_index_assoc _ _ _ _ _ _ inv E E') as (k & Hk & Hk').
-     simpl in *. now rewrite Hk, Hk'.
-   + rewrite <- list_assoc_index_none in E, E'.
-     simpl in *. now rewrite E,E'.
- - destruct list_index; easy.
- - destruct list_index; easy.
- - intros [= <- E]. f_equal.
-   simpl in inv.
-   clear f. revert a a' E inv.
-   fix IH' 1. destruct a as [|t a], a' as [|t' a']; try easy.
+ induction f; destruct f'; intros sub sub'; simpl; intros IV; try easy.
+ - rewrite lazy_andb_iff, !eqb_eq.
+   assert (H := nam2mix_term_ok sub sub' (Nam.Fun "" l) (Nam.Fun "" l0) IV).
    simpl.
-   intros [= E E'] inv. f_equal.
-   + apply IH; auto.
-     eapply Inv_weak; eauto. varsdec.
-   + apply IH'; auto.
-     eapply Inv_weak; eauto. varsdec.
+   split.
+   + intros (<-,E). f_equal. injection (proj1 H); simpl; f_equal; auto.
+   + intros [= <- E]. split; auto. injection (proj2 H); simpl; f_equal; auto.
+ - rewrite IHf by auto.
+   split; [intros <- | intros [=]]; easy.
+ - rewrite !lazy_andb_iff, !eqb_eq.
+   rewrite IHf1, IHf2 by (eapply Inv_weak; eauto; varsdec).
+   split; [intros ((<-,<-),<-)|intros [= <- <- <-]]; easy.
+ - rewrite lazy_andb_iff, !eqb_eq.
+   set (vars := Vars.union _ _).
+   assert (Hz := fresh_var_ok vars).
+   set (z := fresh_var vars) in *.
+   rewrite IHf by (constructor; try (eapply Inv_weak; eauto); varsdec).
+   simpl.
+   split; [intros (<-,<-) | intros [=]]; easy.
 Qed.
 
-Lemma nam2mix_alpha_gen sub sub' f f' :
- Inv (Vars.union (Nam.allvars f) (Nam.allvars f')) sub sub' ->
- nam2mix (map fst sub) f = nam2mix (map fst sub') f' ->
- Nam.alpha_equiv_gen sub f sub' f' = true.
+Lemma nam2mix_canonical (f f' : Nam.formula) :
+ nam2mix [] f = nam2mix [] f' <-> AlphaEq f f'.
 Proof.
- revert f' sub sub'.
- induction f; destruct f'; intros sub sub'; simpl; try easy.
- - case eqbspec; [ intros <- | congruence ].
-   case eqbspec; auto.
-   intros NE inv [=]. destruct NE.
-   injection (nam2mix_term_ok2 sub sub' (Nam.Fun "" l) (Nam.Fun "" l0)); auto.
-   simpl. now f_equal.
- - intros inv [=]. auto.
- - case eqbspec; [ intros <- | congruence].
-   rewrite lazy_andb_iff. intros inv [=]. split.
-   + apply IHf1; auto. eapply Inv_weak; eauto; varsdec.
-   + apply IHf2; auto. eapply Inv_weak; eauto; varsdec.
- - match goal with
-     |- context [fresh_var ?vs] => set (vars := vs)
-   end.
-   case eqbspec; [intros <- | congruence].
-   intros inv [=]. apply IHf; auto.
-   assert (Fok := fresh_var_ok vars).
-   constructor; try (eapply Inv_weak; eauto); varsdec.
+ symmetry. now apply nam2mix_canonical_gen.
 Qed.
 
-Lemma nam2mix_alpha f f' :
-  nam2mix [] f = nam2mix [] f' -> Nam.AlphaEq f f'.
-Proof.
- intros. apply nam2mix_alpha_gen; auto.
-Qed.
-
-Lemma nam2mix_iff f f' :
- nam2mix [] f = nam2mix [] f' <-> Nam.AlphaEq f f'.
-Proof.
- split; auto using nam2mix_alpha, Nam2MixProof.nam2mix_canonical.
-Qed.
-
-End Nam2MixProof.
-
-Fixpoint mix2nam_term stack t :=
-  match t with
-  | Mix.FVar v => Nam.Var v
-  | Mix.BVar n => Nam.Var (List.nth n stack EmptyString)
-  | Mix.Fun f args =>
-    Nam.Fun f (List.map (mix2nam_term stack) args)
-  end.
-
-Fixpoint mix2nam stack f :=
-  match f with
-  | Mix.True => Nam.True
-  | Mix.False => Nam.False
-  | Mix.Not f => Nam.Not (mix2nam stack f)
-  | Mix.Op o f1 f2 =>
-    Nam.Op o (mix2nam stack f1) (mix2nam stack f2)
-  | Mix.Pred p args =>
-    Nam.Pred p (List.map (mix2nam_term stack) args)
-  | Mix.Quant q f =>
-    let v := fresh_var (Vars.union (vars_of_list stack) (Mix.fvars f)) in
-    Nam.Quant q v (mix2nam (v::stack) f)
-  end.
+(** Proofs about [mix2nam] *)
 
 Lemma mix_nam_mix_term stack t :
  NoDup stack ->
- (Mix.level t <= List.length stack)%nat ->
+ Mix.level t <= List.length stack ->
  (forall v, In v stack -> ~Vars.In v (Mix.fvars t)) ->
  nam2mix_term stack (mix2nam_term stack t) = t.
 Proof.
@@ -328,7 +280,7 @@ Qed.
 
 Lemma mix_nam_mix_gen stack f :
  NoDup stack ->
- (Mix.level f <= List.length stack)%nat ->
+ Mix.level f <= List.length stack ->
  (forall v, In v stack -> ~Vars.In v (Mix.fvars f)) ->
  nam2mix stack (mix2nam stack f) = f.
 Proof.
@@ -369,7 +321,7 @@ Proof.
 Qed.
 
 Lemma nam2mix_term_level stack t :
-  (Mix.level (nam2mix_term stack t) <= List.length stack)%nat.
+  Mix.level (nam2mix_term stack t) <= List.length stack.
 Proof.
  revert t.
  fix IH 1. destruct t; cbn.
@@ -381,7 +333,7 @@ Proof.
 Qed.
 
 Lemma nam2mix_level stack f :
-  (Mix.level (nam2mix stack f) <= List.length stack)%nat.
+  Mix.level (nam2mix stack f) <= List.length stack.
 Proof.
  revert stack.
  induction f; intros stack; cbn; auto with arith.
@@ -399,380 +351,26 @@ Qed.
 
 
 Lemma nam_mix_nam f :
-  Nam.AlphaEq (mix2nam [] (nam2mix [] f)) f.
+  AlphaEq (mix2nam [] (nam2mix [] f)) f.
 Proof.
- apply Nam2MixProof.nam2mix_iff.
+ apply nam2mix_canonical.
  apply mix_nam_mix.
  apply nam2mix_closed.
 Qed.
 
 Lemma AlphaEq_equivalence :
-  Equivalence Nam.AlphaEq.
+  Equivalence AlphaEq.
 Proof.
  constructor.
- - intros f. now apply Nam2MixProof.nam2mix_iff.
- - intros f f'. rewrite <-!Nam2MixProof.nam2mix_iff. auto.
- - intros f1 f2 f3. rewrite <-!Nam2MixProof.nam2mix_iff. apply eq_trans.
+ - intros f. now apply nam2mix_canonical.
+ - intros f f'. rewrite <-!nam2mix_canonical. auto.
+ - intros f1 f2 f3. rewrite <-!nam2mix_canonical. apply eq_trans.
 Qed.
 
 Lemma nam2mix_eqb (f f' : Nam.formula) :
  (nam2mix [] f =? nam2mix [] f') = (f =? f').
 Proof.
- case eqbspec; rewrite Nam2MixProof.nam2mix_iff.
+ case eqbspec; rewrite nam2mix_canonical.
  - apply eq_sym.
  - intros H. symmetry. exact (not_true_is_false _ H).
 Qed.
-
-(* TODO
-
-(** Equivalence between form_subst and form_subst',
-    between alpha_equiv and alpha_equiv' *)
-
-Lemma alpha_equiv_genalt sub1 f1 sub2 f2 h :
- Nam.form_height f1 < h -> Nam.form_height f2 < h ->
- Nam.alpha_equiv_gen sub1 f1 sub2 f2 =
- Nam.alpha_equiv_h (Nam.form_substs sub1 f1) (Nam.form_substs sub2 f2) h.
-Proof.
- revert h f1 f2 sub1 sub2.
- induction h.
- - inversion 1.
- - destruct f1; destruct f2; intros sub1 sub2 Hf1 Hf2; auto;
-    try (cbn; now destruct negb).
-   + cbn. apply IHh; auto with arith.
-   + cbn in *. case eqb; auto. rewrite <-!andb_lazy_alt.
-     f_equal; apply IHh; omega with *.
-   + simpl Nam.alpha_equiv_gen.
-     set (z1 := fresh_var _).
-     simpl Nam.form_substs.
-     set (cond1 := negb _).
-     set (cond2 := negb _).
-*)
-
-
-
-
-(** Contexts *)
-
-Definition nam2mix_ctx (c:Nam.context) : Mix.context :=
- List.map (nam2mix []) c.
-
-Definition mix2nam_ctx (c:Mix.context) : Nam.context :=
- List.map (mix2nam []) c.
-
-Lemma nam2mix_ctx_eqb (c c' : Nam.context) :
- (nam2mix_ctx c =? nam2mix_ctx c') = (c =? c').
-Proof.
- revert c'.
- induction c; destruct c'; cbn; auto.
- rewrite nam2mix_eqb. case eqb; auto.
-Qed.
-
-(** Sequents *)
-
-Definition nam2mix_seq '(Nam.Seq c f) : Mix.sequent :=
-  Mix.Seq (nam2mix_ctx c) (nam2mix [] f).
-
-Definition mix2nam_seq '(Mix.Seq c f) : Nam.sequent :=
-  Nam.Seq (mix2nam_ctx c) (mix2nam [] f).
-
-Lemma nam2mix_seq_eqb (s s' : Nam.sequent) :
- (nam2mix_seq s =? nam2mix_seq s') = (s =? s').
-Proof.
- destruct s as (c,f), s' as (c',f'); cbn.
- now rewrite nam2mix_ctx_eqb, nam2mix_eqb.
-Qed.
-
-
-(** Rule kinds *)
-
-Definition nam2mix_rule r :=
-  match r with
-  | Nam.Ax => Mix.Ax
-  | Nam.Tr_i => Mix.Tr_i
-  | Nam.Fa_e => Mix.Fa_e
-  | Nam.Not_i => Mix.Not_i
-  | Nam.Not_e => Mix.Not_e
-  | Nam.And_i => Mix.And_i
-  | Nam.And_e1 => Mix.And_e1
-  | Nam.And_e2 => Mix.And_e2
-  | Nam.Or_i1 => Mix.Or_i1
-  | Nam.Or_i2 => Mix.Or_i2
-  | Nam.Or_e => Mix.Or_e
-  | Nam.Imp_i => Mix.Imp_i
-  | Nam.Imp_e => Mix.Imp_e
-  | Nam.All_i v => Mix.All_i v
-  | Nam.All_e t => Mix.All_e (nam2mix_term [] t)
-  | Nam.Ex_i t => Mix.Ex_i (nam2mix_term [] t)
-  | Nam.Ex_e v => Mix.Ex_e v
-  | Nam.Absu => Mix.Absu
-  end.
-
-Definition mix2nam_rule r :=
-  match r with
-  | Mix.Ax => Nam.Ax
-  | Mix.Tr_i => Nam.Tr_i
-  | Mix.Fa_e => Nam.Fa_e
-  | Mix.Not_i => Nam.Not_i
-  | Mix.Not_e => Nam.Not_e
-  | Mix.And_i => Nam.And_i
-  | Mix.And_e1 => Nam.And_e1
-  | Mix.And_e2 => Nam.And_e2
-  | Mix.Or_i1 => Nam.Or_i1
-  | Mix.Or_i2 => Nam.Or_i2
-  | Mix.Or_e => Nam.Or_e
-  | Mix.Imp_i => Nam.Imp_i
-  | Mix.Imp_e => Nam.Imp_e
-  | Mix.All_i v => Nam.All_i v
-  | Mix.All_e t => Nam.All_e (mix2nam_term [] t)
-  | Mix.Ex_i t => Nam.Ex_i (mix2nam_term [] t)
-  | Mix.Ex_e v => Nam.Ex_e v
-  | Mix.Absu => Nam.Absu
-  end.
-
-(** Derivations *)
-
-Fixpoint nam2mix_deriv (d:Nam.derivation) :=
-  let '(Nam.Rule r s ds) := d in
-  Mix.Rule
-    (nam2mix_rule r)
-    (nam2mix_seq s)
-    (List.map nam2mix_deriv ds).
-
-Fixpoint mix2nam_deriv (d:Mix.derivation) :=
-  let '(Mix.Rule r s ds) := d in
-  Nam.Rule
-    (mix2nam_rule r)
-    (mix2nam_seq s)
-    (List.map mix2nam_deriv ds).
-
-Ltac break :=
- rewrite <- ?andb_lazy_alt;
- match goal with
- | |- _ = match ?f ?x with _ => _ end => destruct x
- | |- _ = match ?x with _ => _ end => destruct x
- | |- match ?f (?g ?x) with _ => _ end = _ => destruct x
- | |- match ?f ?x with _ => _ end = _ => destruct x
- | |- match ?x with _ => _ end = _ => destruct x
- end.
-
-Lemma lazy_andb_false (a:bool) : a &&& false = false.
-Proof.
- now destruct a.
-Qed.
-
-(*
-Lemma subst_equiv (sub:Nam.subst) f v z q :
- ~Vars.In z (Vars.union (Nam.allvars f) (Nam.subvars sub)) ->
- Nam.AlphaEq
-   (Nam.formula_substs sub (Nam.Quant q v f))
-   (Nam.Quant q z (Nam.formula_substs ((v,Nam.Var z)::sub) f)).
-Proof.
- unfold Nam.AlphaEq, Nam.alpha_equiv.
- intros NI.
- cbn -[fresh_var Vars.union].
- set (cond := negb _).
- destruct cond eqn:Hcond.
- - cbn -[fresh_var Vars.union].
-   set (z' := fresh_var _).
-   rewrite eqb_refl.
-*)
-
-(*
-Lemma nam2mix_term_subts
-forall a : Nam.term,
-  In a l ->
-  nam2mix_term (map snd subvar)
-    (Nam.term_substs
-       (map (fun '(v0, w) => (v0, Nam.Var w)) subvar ++
-        [(v, t)]) a) =
-  Mix.bsubst n (nam2mix_term [] t)
-    (nam2mix_term (map fst subvar ++ [v]) a)
-*)
-
-Definition subvar2sub (subvar:list (variable*variable)) :=
-  List.map (fun '(v,w) => (v,Nam.Var w)) subvar.
-
-(*TODO
-
-Lemma nam2mix_term_substs_ext
- (vars:list variable)
- (subvar subvar' : list (variable*variable))
- (sub : Nam.subst) t :
-  (forall v, list_assoc_dft v subvar v = list_assoc_dft v subvar' v) ->
-  nam2mix_term (List.map (fun v => list_assoc_dft v subvar v) vars)
-          (Nam.term_substs (subvar2sub subvar ++ sub) t) =
-  nam2mix_term (List.map (fun v => list_assoc_dft v subvar' v) vars)
-          (Nam.term_substs (subvar2sub subvar' ++ sub) t).
-Proof.
- induction t as [v|f l IH] using Nam.term_ind'; intros E.
- - cbn.
-
-
-Lemma nam2mix_substs_ext
- (vars:list variable)
- (subvar subvar' : list (variable*variable))
- (sub : Nam.subst) f :
-  (forall v, subvar v = subvar') ->
-  nam2mix (List.map (fun v => list_assoc_dft v subvar v) vars)
-          (Nam.formula_substs (subvar2sub subvar ++ sub) f) =
-  nam2mix (List.map (fun v => list_assoc_dft v subvar' v) vars)
-          (Nam.formula_substs (subvar2sub subvar' ++ sub) f).
-Proof.
- revert vars subvar subvar' sub.
- induction f; intros var subvar subvar' sub.
- - now cbn.
- - now cbn.
- - cbn. f_equal. rewrite !map_map. apply map_ext.
-
-
-Definition InvSubVar v t f subvar :=
-  ~In v (List.map fst subvar) /\ ~In v (List.map snd subvar) /\
-   (forall w, In w (List.map snd subvar) ->
-              ~Vars.In w (Vars.union (Nam.term_vars t) (Nam.allvars f))).
-
-Lemma nam2mix_substs n (subvar: list (variable*variable)) v t f :
-  InvSubVar v t f subvar ->
-  n = List.length subvar ->
-  let sub := List.map (fun '(v,w) => (v,Nam.Var w)) subvar
-  in
-  nam2mix (List.map snd subvar) (Nam.formula_substs (sub++[(v,t)]) f) =
-  Mix.bsubst n (nam2mix_term [] t)
-    (nam2mix ((List.map fst subvar) ++ [v]) f).
-Proof.
- revert n subvar.
- induction f; cbn -[fresh_var Vars.union]; trivial.
- - intros.
-   f_equal.
-   rewrite !map_map.
-   apply map_ext_in.
-   admit.
- - intros. f_equal; auto.
- - intros. f_equal; auto. admit. admit.
- - intros.
-   set (cond := negb _).
-   destruct cond eqn:Hcond.
-   + cbn. f_equal.
-     set (sub := filter _ _) in *.
-     specialize (IHf (S n) ((v0,v0)::subvar)).
-     cbn in IHf. rewrite <- IHf; auto.
-     case (eqbspec v v0).
-     * intros <-.
-       assert (sub = map (fun '(v, w) => (v, Nam.Var w)) subvar).
-       { admit. }
-
-     *
-
-     admit.
-   + set (sub := filter _ _) in *.
-     set (z := fresh_var _).
-     cbn -[z].
-     f_equal.
-     specialize (IHf (S n) ((v0,z)::subvar)).
-     cbn in IHf. rewrite <- IHf; auto.
-     admit.
-
-Lemma nam2mix_subst v t f :
-  nam2mix [] (Nam.formula_subst v t f) =
-  Mix.bsubst 0 (nam2mix_term [] t) (nam2mix [v] f).
-Proof.
-Admitted. (* preuve ??? *)
-
-
-Lemma nam2mix_deriv_valid_step logic (d:Nam.derivation) :
-  Mix.valid_deriv_step logic (nam2mix_deriv d) =
-  Nam.valid_deriv_step logic d.
-Proof.
- destruct d as [[ ] s ds]; cbn.
- - repeat (break; cbn; auto).
-   unfold nam2mix_ctx.
-   induction c as [|A c IH]; cbn; auto.
-   rewrite <- nam2mix_eqb.
-   case eqbspec; auto.
- - repeat (break; cbn; auto).
- - repeat (break; cbn; auto).
-   rewrite <- !nam2mix_seq_eqb. now destruct d.
- - repeat (break; cbn; auto).
-   rewrite <- !nam2mix_seq_eqb. now destruct d.
- - repeat (break; cbn; auto).
-   now rewrite nam2mix_eqb, !nam2mix_ctx_eqb.
- - repeat (break; cbn; auto).
-   rewrite <- !nam2mix_seq_eqb. now destruct d, d0.
- - repeat (break; cbn; auto).
-   now rewrite <- !nam2mix_seq_eqb.
- - repeat (break; cbn; auto).
-   now rewrite <- !nam2mix_seq_eqb.
- - repeat (break; cbn; auto).
-   rewrite <- !nam2mix_seq_eqb. now destruct d.
- - repeat (break; cbn; auto).
-   rewrite <- !nam2mix_seq_eqb. now destruct d.
- - repeat (break; cbn; auto).
-   rewrite <- nam2mix_ctx_eqb, <- !nam2mix_seq_eqb.
-   now destruct d, d0.
- - repeat (break; cbn; auto).
-   rewrite <- nam2mix_seq_eqb. now destruct d.
- - repeat (break; cbn; auto).
-   rewrite <- !nam2mix_seq_eqb. now destruct d.
- - repeat (break; cbn - [Nam.alpha_equiv]; auto);
-    rewrite ?andb_false_r; auto.
-   rewrite <- nam2mix_ctx_eqb.
-   case eqbspec; auto. intro Ec. simpl.
-   rewrite <- nam2mix_eqb. cbn.
-   apply eq_true_iff_eq. simpl.
-   rewrite !andb_true_iff.
-   rewrite !negb_true_iff, <- !not_true_iff_false.
-   rewrite !Vars.mem_spec.
-   rewrite !eqb_eq.
-   split; intros (U,V); split.
-   + change (Mix.FVar x) with (nam2mix_term [] (Nam.Var x)) in U.
-     rewrite <- nam2mix_subst in U.
-     (* f est f0 avec des x à la place des v, donc credible *)
-       admit.
-   + (* faut montrer que c equiv c0 -> memes variables libres *)
-       admit.
-   + rewrite U.
-     change (Mix.FVar x) with (nam2mix_term [] (Nam.Var x)).
-     rewrite <- nam2mix_subst.
-     (* TODO:
-        alpha_equiv (Nam.formula_subst x (Nam.Var x) f) f
-       *)
-       admit.
-   + (* - memes variables libres dans contextes equivs
-          - nam2mix [x] f0 n'a pas x comme variable libre... *)
-       admit.
- - repeat (break; cbn; auto).
-   rewrite !nam2mix_ctx_eqb. case eqb; simpl; auto.
-   rewrite <- nam2mix_eqb.
-   now rewrite <- nam2mix_subst.
- - repeat (break; cbn; auto).
-   rewrite !nam2mix_ctx_eqb. case eqb; simpl; auto.
-   rewrite <- nam2mix_eqb.
-   now rewrite <- nam2mix_subst.
- - repeat (break; cbn - [Nam.alpha_equiv]; auto);
-    rewrite ?andb_false_r; auto.
-   rewrite <- nam2mix_seq_eqb, <- nam2mix_eqb. cbn.
-   apply eq_true_iff_eq.
-   rewrite !andb_true_iff.
-   rewrite !negb_true_iff, <- !not_true_iff_false.
-   rewrite !Vars.mem_spec.
-   rewrite !eqb_eq.
-   split.
-   + intros (((U,V),W),X); repeat split.
-     * rewrite <-V in U; exact U.
-     * rewrite <- nam2mix_ctx_eqb. now apply eqb_eq.
-     * admit. (* bsubst... *)
-     * destruct s. cbn in *. injection U as U U'. admit.
-   + intros ((U,(V,W)),Z); repeat split.
-     * rewrite <- nam2mix_ctx_eqb in V. apply eqb_eq in V.
-       rewrite U. f_equal; auto.
-     * rewrite <- nam2mix_ctx_eqb in V. apply eqb_eq in V.
-       rewrite V. auto.
-     * rewrite W.
-       change (Mix.FVar x) with (nam2mix_term [] (Nam.Var x)).
-       rewrite <- nam2mix_subst.
-       admit.
-     * destruct s. cbn in *. injection U as U U'. admit.
- - repeat (break; cbn; auto).
-   case eqb; simpl; auto.
-   now rewrite <- nam2mix_seq_eqb.
-Admitted.
-*)
